ExistentialRules/Triggers/Basic.lean
@@ -6,16 +6,68 @@ structure PreTrigger (sig : Signature) [DecidableEq sig.P] [DecidableEq sig.C] [
   subs : GroundSubstitution sig
 
 namespace PreTrigger
+
   variable {sig : Signature} [DecidableEq sig.P] [DecidableEq sig.C] [DecidableEq sig.V]
 
   def skolemize_var_or_const (trg : PreTrigger sig) (disjunctIndex : Nat) (var_or_const : VarOrConst sig) : SkolemTerm sig :=
     var_or_const.skolemize trg.rule.id disjunctIndex trg.rule.frontier
 
-  def apply_to_skolemized_term (trg : PreTrigger sig) (skolem_term : SkolemTerm sig) : GroundTerm sig :=
-    trg.subs.apply_skolem_term skolem_term
-
   def apply_to_var_or_const (trg : PreTrigger sig) (disjunctIndex : Nat) : VarOrConst sig -> GroundTerm sig :=
-    (trg.apply_to_skolemized_term ∘ (trg.skolemize_var_or_const disjunctIndex))
+    (trg.subs.apply_skolem_term ∘ (trg.skolemize_var_or_const disjunctIndex))
+
+  theorem apply_to_var_or_const_for_const (trg : PreTrigger sig) (i : Nat) :
+      ∀ c, trg.apply_to_var_or_const i (.const c) = GroundTerm.const c := by
+    simp [apply_to_var_or_const, skolemize_var_or_const, VarOrConst.skolemize, GroundSubstitution.apply_skolem_term]
+
+  theorem apply_to_var_or_const_frontier_var (trg : PreTrigger sig) (i : Nat) :
+      ∀ v, v ∈ trg.rule.frontier -> trg.apply_to_var_or_const i (.var v) = trg.subs v := by
+    intro v v_front
+    simp [apply_to_var_or_const, skolemize_var_or_const, VarOrConst.skolemize, v_front, GroundSubstitution.apply_skolem_term]
+
+  def functional_term_for_var (trg : PreTrigger sig) (i : Nat) (v : sig.V) : GroundTerm sig :=
+    GroundTerm.func
+      { ruleId := trg.rule.id, disjunctIndex := i, var := v, arity := trg.rule.frontier.length }
+      (trg.rule.frontier.map trg.subs)
+      (by rw [List.length_map])
+
+  theorem apply_to_var_or_const_non_frontier_var (trg : PreTrigger sig) (i : Nat) :
+      ∀ v, ¬ v ∈ trg.rule.frontier -> trg.apply_to_var_or_const i (.var v) =
+        trg.functional_term_for_var i v := by
+    intro v v_front
+    simp [functional_term_for_var, apply_to_var_or_const, skolemize_var_or_const, VarOrConst.skolemize, v_front, GroundSubstitution.apply_skolem_term]
+
+  theorem apply_to_var_or_const_injective_of_not_in_frontier {v : sig.V}
+      (trg : PreTrigger sig) (i : Fin trg.rule.head.length) (v_not_in_frontier : ¬ v ∈ trg.rule.frontier) :
+      ∀ voc, (trg.apply_to_var_or_const i (VarOrConst.var v)) = (trg.apply_to_var_or_const i voc) ->
+      VarOrConst.var v = voc := by
+    intro voc apply_eq
+    unfold apply_to_var_or_const at apply_eq
+    simp only [Function.comp_apply] at apply_eq
+
+    cases voc with
+    | const c =>
+      simp [GroundSubstitution.apply_skolem_term, skolemize_var_or_const, VarOrConst.skolemize, v_not_in_frontier, GroundTerm.func, GroundTerm.const] at apply_eq
+    | var u =>
+      cases Decidable.em (u ∈ trg.rule.frontier) with
+      | inl u_front =>
+        simp [GroundSubstitution.apply_skolem_term, skolemize_var_or_const, VarOrConst.skolemize, v_not_in_frontier, u_front, GroundTerm.func] at apply_eq
+        rw [Subtype.mk.injEq] at apply_eq
+        apply False.elim
+        apply FiniteTree.tree_eq_while_contained_is_impossible _ _ _ apply_eq
+        rw [FiniteTreeList.fromListToListIsId]
+        unfold List.unattach
+        rw [List.map_map, List.mem_map]
+        exists u
+      | inr u_front =>
+        apply VarOrConst.skolemize_injective trg.rule.id i trg.rule.frontier
+        apply trg.subs.apply_skolem_term_injective_on_func_of_frontier_eq
+        . unfold VarOrConst.skolemize
+          simp only [v_not_in_frontier, u_front, ↓reduceIte]
+          rfl
+        . unfold VarOrConst.skolemize
+          simp only [v_not_in_frontier, u_front, ↓reduceIte]
+          rfl
+        . exact apply_eq
 
   def apply_to_function_free_atom (trg : PreTrigger sig) (disjunctIndex : Nat) (atom : FunctionFreeAtom sig) : Fact sig :=
     {
@@ -37,309 +89,183 @@ namespace PreTrigger
     unfold mapped_head
     rw [List.length_map, List.length_enum]
 
-  -- TODO: remove this and use mapped_head directly
-  def result (trg : PreTrigger sig) : List (FactSet sig) :=
-    trg.mapped_head.map List.toSet
-
-  theorem subs_application_is_injective_for_freshly_introduced_terms {t : sig.V} (trg : PreTrigger sig) (disjunctIndex : Fin trg.rule.head.length) (t_not_in_frontier : ¬ t ∈ trg.rule.frontier) : ∀ s, (trg.apply_to_var_or_const disjunctIndex (VarOrConst.var t) = trg.apply_to_var_or_const disjunctIndex (VarOrConst.var s)) -> trg.skolemize_var_or_const disjunctIndex (VarOrConst.var t) = trg.skolemize_var_or_const disjunctIndex (VarOrConst.var s) := by
-    intro s apply_eq_for_t_and_s
-
-    cases Decidable.em (s ∈ trg.rule.frontier) with
-    | inr hr =>
-      simp [GroundTerm.func, t_not_in_frontier, hr, apply_to_var_or_const, apply_to_skolemized_term, skolemize_var_or_const, GroundSubstitution.apply_skolem_term, VarOrConst.skolemize] at apply_eq_for_t_and_s
-      simp [t_not_in_frontier, hr, apply_to_var_or_const, apply_to_skolemized_term, skolemize_var_or_const, GroundSubstitution.apply_skolem_term, VarOrConst.skolemize]
-      exact apply_eq_for_t_and_s
-    | inl hl =>
-      simp [GroundTerm.func, t_not_in_frontier, hl, apply_to_var_or_const, apply_to_skolemized_term, skolemize_var_or_const, GroundSubstitution.apply_skolem_term, VarOrConst.skolemize] at apply_eq_for_t_and_s
-      apply False.elim
-      let tree_for_s := trg.apply_to_var_or_const disjunctIndex (VarOrConst.var s)
-      let ts := trg.rule.frontier.map (fun fv => trg.subs fv)
-      let a : SkolemFS sig := { ruleId := trg.rule.id, disjunctIndex, var := t, arity := trg.rule.frontier.length }
-      apply FiniteTree.tree_eq_while_contained_is_impossible tree_for_s (FiniteTreeList.fromList ts.unattach) a
-      . simp [tree_for_s, apply_to_var_or_const, apply_to_skolemized_term, skolemize_var_or_const, GroundSubstitution.apply_skolem_term, VarOrConst.skolemize, hl]
-        rw [← apply_eq_for_t_and_s]
-      simp [tree_for_s, apply_to_var_or_const, apply_to_skolemized_term, skolemize_var_or_const, GroundSubstitution.apply_skolem_term, VarOrConst.skolemize, hl]
-      rw [FiniteTreeList.fromListToListIsId]
-      unfold List.unattach
-      unfold ts
-      rw [List.map_map, List.mem_map]
-      exists s
-
-  def idx_of_fact_in_result (trg : PreTrigger sig) (f : Fact sig) (disj_index : Fin trg.result.length) (f_in_res : f ∈ trg.result.get disj_index) : Fin (trg.rule.head.get ⟨disj_index.val, (by rw [← length_mapped_head]; have isLt := disj_index.isLt; unfold result at isLt; simp only [List.length_map] at isLt; exact isLt)⟩).length :=
-    let disj_index_mapped_head : Fin trg.mapped_head.length := ⟨disj_index.val, (by have isLt := disj_index.isLt; unfold result at isLt; simp only [List.length_map] at isLt; exact isLt)⟩
-    let fin_mapped := (trg.mapped_head.get disj_index_mapped_head).idx_of (((trg.mapped_head.get disj_index_mapped_head).mem_toSet (e := f)).mp (by unfold result at f_in_res; simp at f_in_res; apply f_in_res))
-    have fin_mapped_isLt := fin_mapped.isLt
-    ⟨fin_mapped.val, by simp [mapped_head] at fin_mapped_isLt; exact fin_mapped_isLt⟩
-
-  theorem apply_subs_to_atom_at_idx_same_as_fact_at_idx (trg : PreTrigger sig) (disj_index : Fin trg.rule.head.length) (idx : Fin (trg.rule.head.get disj_index).length) : trg.apply_to_function_free_atom disj_index ((trg.rule.head.get disj_index).get idx) = (trg.mapped_head.get ⟨disj_index.val, (by rw [length_mapped_head]; exact disj_index.isLt)⟩).get ⟨idx.val, (by unfold mapped_head; simp)⟩ := by
+  theorem length_each_mapped_head (trg : PreTrigger sig) : ∀ (n : Nat), trg.mapped_head[n]?.map (List.length) = trg.rule.head[n]?.map (List.length) := by
+    intro n
     unfold mapped_head
-    simp
+    simp only [List.getElem?_map, List.getElem?_enum, Option.map_map]
+    cases trg.rule.head[n]? <;> simp
+
+  def subs_for_mapped_head (trg : PreTrigger sig) (i : Fin trg.mapped_head.length) : GroundSubstitution sig :=
+    fun v => trg.apply_to_var_or_const i (.var v)
+
+  theorem apply_subs_for_var_or_const_eq (trg : PreTrigger sig) (i : Fin trg.mapped_head.length) :
+      ∀ voc, (trg.subs_for_mapped_head i).apply_var_or_const voc = trg.apply_to_var_or_const i voc := by
+    intro voc
+    unfold GroundSubstitution.apply_var_or_const
+    unfold subs_for_mapped_head
+    unfold apply_to_var_or_const
+    cases voc <;> simp [skolemize_var_or_const, VarOrConst.skolemize, GroundSubstitution.apply_skolem_term]
+
+  theorem apply_subs_for_atom_eq (trg : PreTrigger sig) (i : Fin trg.mapped_head.length) :
+      ∀ a, (trg.subs_for_mapped_head i).apply_function_free_atom a = trg.apply_to_function_free_atom i a := by
+    intro a
+    unfold GroundSubstitution.apply_function_free_atom
+    unfold apply_to_function_free_atom
+    simp only [Fact.mk.injEq, true_and]
+    rw [List.map_inj_left]
+    intros
+    apply apply_subs_for_var_or_const_eq
+
+  theorem apply_subs_for_mapped_head_eq (trg : PreTrigger sig) (i : Fin trg.mapped_head.length) :
+      (trg.subs_for_mapped_head i).apply_function_free_conj (trg.rule.head[i.val]'(by rw [← length_mapped_head]; exact i.isLt)) =
+      trg.mapped_head[i.val] := by
+    unfold mapped_head
+    unfold subs_for_mapped_head
+    unfold GroundSubstitution.apply_function_free_conj
+    rw [List.getElem_map, List.getElem_enum, List.map_inj_left]
+    intros
+    apply apply_subs_for_atom_eq trg i
+
+  def atom_for_result_fact (trg : PreTrigger sig) {f : Fact sig} (i : Fin trg.mapped_head.length)
+      (f_mem : f ∈ trg.mapped_head[i.val]) : FunctionFreeAtom sig :=
+    let j := trg.mapped_head[i.val].idx_of f_mem
+    let i' : Fin trg.rule.head.length := ⟨i.val, by rw [← length_mapped_head]; exact i.isLt⟩
+    let j' : Fin (trg.rule.head[i'.val].length) := ⟨j.val, by
+      have := trg.length_each_mapped_head i.val
+      rw [List.getElem?_eq_getElem i.isLt] at this
+      rw [List.getElem?_eq_getElem i'.isLt] at this
+      simp only [Option.map_some', Option.some_inj] at this
+      rw [← this]
+      exact j.isLt
+    ⟩
+    trg.rule.head[i'.val][j'.val]
+
+  theorem apply_on_atom_for_result_fact_is_fact (trg : PreTrigger sig) {f : Fact sig} (i : Fin trg.mapped_head.length)
+      (f_mem : f ∈ trg.mapped_head[i.val]) : trg.apply_to_function_free_atom i (trg.atom_for_result_fact i f_mem) = f := by
+    have : f = trg.mapped_head[i.val].get (trg.mapped_head[i.val].idx_of f_mem) := by apply List.idx_of_get
+    rw [List.get_eq_getElem] at this
+    conv => right; rw [this]
+    unfold mapped_head
+    unfold atom_for_result_fact
+    simp only [List.getElem_map, List.getElem_enum]
+
+  def var_or_const_for_result_term (trg : PreTrigger sig) {f : Fact sig} {t : GroundTerm sig} (i : Fin trg.mapped_head.length)
+      (f_mem : f ∈ trg.mapped_head[i.val]) (t_mem : t ∈ f.terms) : VarOrConst sig :=
+    let k := f.terms.idx_of t_mem
+    let atom := trg.atom_for_result_fact i f_mem
+    let k' : Fin atom.terms.length := ⟨k.val, by
+      have isLt := k.isLt
+      have := trg.apply_on_atom_for_result_fact_is_fact i f_mem
+      conv at isLt => right; rw [← this]
+      unfold apply_to_function_free_atom at isLt
+      rw [List.length_map] at isLt
+      exact isLt
+    ⟩
+    atom.terms[k']
+
+  theorem apply_on_var_or_const_for_result_term_is_term (trg : PreTrigger sig) {f : Fact sig} {t : GroundTerm sig}
+      (i : Fin trg.mapped_head.length) (f_mem : f ∈ trg.mapped_head[i.val]) (t_mem : t ∈ f.terms) :
+      trg.apply_to_var_or_const i (trg.var_or_const_for_result_term i f_mem t_mem) = t := by
+    have t_eq : t = f.terms.get (f.terms.idx_of t_mem) := by apply List.idx_of_get
+    rw [List.get_eq_getElem] at t_eq
+    have := trg.apply_on_atom_for_result_fact_is_fact i f_mem
+    have : (trg.apply_to_function_free_atom i (trg.atom_for_result_fact i f_mem)).terms = f.terms := by rw [this]
+    conv at t_eq => right; simp only [← this]
+    conv => right; rw [t_eq]
+    unfold apply_to_function_free_atom
+    rw [List.getElem_map]
+    unfold var_or_const_for_result_term
+    rfl
 
   def loaded (trg : PreTrigger sig) (F : FactSet sig) : Prop :=
     trg.mapped_body.toSet ⊆ F
 
-  def satisfied_for_disj (trg : PreTrigger sig) (F : FactSet sig) (disj_index : Fin trg.rule.head.length) : Prop :=
+  theorem term_mapping_preserves_loadedness (trg : PreTrigger sig) (fs : FactSet sig) (h : GroundTermMapping sig) (h_id : h.isIdOnConstants) : trg.loaded fs -> { rule := trg.rule, subs := h ∘ trg.subs : PreTrigger sig }.loaded (h.applyFactSet fs) := by
+    unfold loaded
+    unfold mapped_body
+    intro loaded
+    intro f f_mem
+    rw [List.mem_toSet] at f_mem
+    simp only [GroundSubstitution.apply_function_free_conj] at f_mem
+    rw [List.mem_map] at f_mem
+    rcases f_mem with ⟨a, a_mem, f_mem⟩
+    rw [GroundSubstitution.apply_function_free_atom_compose _ _ h_id] at f_mem
+    rw [← f_mem]
+    apply GroundTermMapping.applyPreservesElement
+    apply loaded
+    unfold GroundSubstitution.apply_function_free_conj
+    rw [List.mem_toSet, List.mem_map]
+    exists a
+
+  def satisfied_for_disj (trg : PreTrigger sig) (fs : FactSet sig) (disj_index : Fin trg.rule.head.length) : Prop :=
     ∃ (s : GroundSubstitution sig),
       (∀ v, v ∈ (Rule.frontier trg.rule) → s v = trg.subs v) ∧
-      ((s.apply_function_free_conj (trg.rule.head.get disj_index)).toSet ⊆ F)
+      ((s.apply_function_free_conj (trg.rule.head[disj_index.val])).toSet ⊆ fs)
+
+  theorem satisfied_for_disj_of_mapped_head_contained (trg : PreTrigger sig) (fs : FactSet sig)
+      (disj_index : Fin trg.rule.head.length) :
+      (trg.mapped_head[disj_index.val]'(by rw [length_mapped_head]; exact disj_index.isLt)).toSet ⊆ fs ->
+      trg.satisfied_for_disj fs disj_index := by
+    intro h
+    let i : Fin trg.mapped_head.length := ⟨disj_index.val, by rw [length_mapped_head]; exact disj_index.isLt⟩
+    exists trg.subs_for_mapped_head i
+    constructor
+    . intro v v_mem; unfold subs_for_mapped_head; rw [trg.apply_to_var_or_const_frontier_var i v v_mem]
+    . rw [trg.apply_subs_for_mapped_head_eq i]; exact h
 
   def satisfied (trg : PreTrigger sig) (F : FactSet sig) : Prop :=
     ∃ disj_index, trg.satisfied_for_disj F disj_index
 
-  theorem term_mapping_preserves_loadedness (trg : PreTrigger sig) (F : FactSet sig) (h : GroundTermMapping sig) (hh : h.isIdOnConstants) : trg.loaded F -> { rule := trg.rule, subs := h ∘ trg.subs : PreTrigger sig }.loaded (h.applyFactSet F) := by
-    simp [loaded, mapped_body]
-    induction trg.rule.body with
-    | nil => intro _ _ _; contradiction
-    | cons head tail ih =>
-      intro base f hf
-      simp [Set.element, Set.union, List.toSet] at hf
-      cases hf with
-      | inl hl =>
-        have := Set.element_mapping_preserves_membership (GroundSubstitution.apply_function_free_atom trg.subs head) F h.applyFact
-        have := this (base (GroundSubstitution.apply_function_free_atom trg.subs head) (by apply Or.inl; simp [Set.element]))
-        simp [Set.element, GroundTermMapping.applyFactSet]
-        simp [Set.element] at this
-        cases this with | intro e he =>
-          exists e
-          rw [hl]
-          constructor
-          exact he.left
-          rw [← he.right]
-          simp [GroundTermMapping.applyFact, GroundSubstitution.apply_function_free_atom]
-          induction head.terms with
-          | nil => simp [List.map]
-          | cons t_head t_tail t_ih =>
-            simp [List.map]
-            constructor
-            . cases t_head with
-              | var v => simp [GroundSubstitution.apply_var_or_const]
-              | const c => simp [GroundSubstitution.apply_var_or_const]; apply hh (GroundTerm.const c)
-            . apply t_ih
-      | inr hr =>
-        apply ih
-        intro _ hf'; apply base; apply Or.inr; apply hf'
-        exact hr
-
   def equiv (trg1 trg2 : PreTrigger sig) : Prop :=
-    trg1.rule = trg2.rule ∧ ∀ v, v ∈ trg1.rule.frontier.toSet -> trg1.subs v = trg2.subs v
+    trg1.rule = trg2.rule ∧ ∀ v, v ∈ trg1.rule.frontier -> trg1.subs v = trg2.subs v
 
-  theorem result_eq_of_equiv (trg1 trg2 : PreTrigger sig) : trg1.equiv trg2 -> trg1.result = trg2.result := by
+  theorem result_eq_of_equiv (trg1 trg2 : PreTrigger sig) : trg1.equiv trg2 -> trg1.mapped_head = trg2.mapped_head := by
     unfold equiv
     intro h
-
-    have : trg1.mapped_head = trg2.mapped_head := by
-      unfold mapped_head
-      rw [h.left]
-      rw [List.map_eq_map_iff]
-      intro _ _
-      unfold PreTrigger.apply_to_function_free_atom
-      simp
-      intro a _ voc hvoc
-      cases voc with
-      | const c => simp [PreTrigger.apply_to_var_or_const, PreTrigger.apply_to_skolemized_term, PreTrigger.skolemize_var_or_const, GroundSubstitution.apply_skolem_term, VarOrConst.skolemize]
-      | var v =>
-        cases Decidable.em (v ∈ trg1.rule.frontier) with
-        | inl v_in_frontier =>
-          simp [PreTrigger.apply_to_var_or_const, PreTrigger.apply_to_skolemized_term, PreTrigger.skolemize_var_or_const, GroundSubstitution.apply_skolem_term]
-          rw [← h.left]
-          simp [VarOrConst.skolemize, v_in_frontier]
-          apply h.right
-          rw [List.mem_toSet]
-          apply v_in_frontier
-        | inr v_not_in_frontier =>
-          simp [PreTrigger.apply_to_var_or_const, PreTrigger.apply_to_skolemized_term, PreTrigger.skolemize_var_or_const, GroundSubstitution.apply_skolem_term]
-          rw [← h.left]
-          simp [GroundTerm.func, VarOrConst.skolemize, v_not_in_frontier]
-          apply congrArg
-          rw [List.eq_iff_unattach_eq]
+    unfold mapped_head
+    rw [h.left]
+    rw [List.map_inj_left]
+    intro e e_mem
+    rw [List.map_inj_left]
+    intro a a_mem
+    unfold apply_to_function_free_atom
+    simp only [Fact.mk.injEq, true_and]
+    rw [List.map_inj_left]
+    intro voc voc_mem
+    cases voc with
+    | const c => simp only [PreTrigger.apply_to_var_or_const_for_const]
+    | var v =>
+      cases Decidable.em (v ∈ trg1.rule.frontier) with
+      | inl v_front =>
+        have v_front_2 : v ∈ trg2.rule.frontier := by rw [← h.left]; exact v_front
+        rw [PreTrigger.apply_to_var_or_const_frontier_var _ _ _ v_front]
+        rw [PreTrigger.apply_to_var_or_const_frontier_var _ _ _ v_front_2]
+        apply h.right
+        exact v_front
+      | inr v_front =>
+        have v_front_2 : ¬ v ∈ trg2.rule.frontier := by rw [← h.left]; exact v_front
+        rw [PreTrigger.apply_to_var_or_const_non_frontier_var _ _ _ v_front]
+        rw [PreTrigger.apply_to_var_or_const_non_frontier_var _ _ _ v_front_2]
+        unfold PreTrigger.functional_term_for_var
+        simp only [← h.left]
+        have : trg1.rule.frontier.map trg1.subs = trg1.rule.frontier.map trg2.subs := by
           rw [List.map_inj_left]
-          intro w hw
-          rw [← h.right w]
-          rw [List.mem_toSet]
-          exact hw
+          exact h.right
+        simp only [this]
 
-    unfold result
-    rw [this]
-
-  theorem result_term_not_in_frontier_image_of_var_not_in_frontier (trg : PreTrigger sig) (disj_index : Fin trg.result.length) (v : sig.V) (v_not_in_frontier : ¬ v ∈ trg.rule.frontier) :
+  theorem result_term_not_in_frontier_image_of_var_not_in_frontier (trg : PreTrigger sig)
+      (disj_index : Fin trg.rule.head.length) (v : sig.V) (v_not_in_frontier : ¬ v ∈ trg.rule.frontier) :
       ¬ trg.apply_to_var_or_const disj_index.val (VarOrConst.var v) ∈ trg.rule.frontier.map trg.subs := by
     intro contra
     apply v_not_in_frontier
-    simp at contra
+    rw [List.mem_map] at contra
     rcases contra with ⟨u, u_in_frontier, u_eq⟩
 
-    have := subs_application_is_injective_for_freshly_introduced_terms trg ⟨disj_index, by rw [← length_mapped_head]; have isLt := disj_index.isLt; unfold result at isLt; simp at isLt; exact isLt⟩ v_not_in_frontier u (by
-      rw [← u_eq]
-      simp [apply_to_var_or_const, skolemize_var_or_const, apply_to_skolemized_term, GroundSubstitution.apply_skolem_term, VarOrConst.skolemize, u_in_frontier]
-    )
-    have : VarOrConst.var v = VarOrConst.var u := by apply VarOrConst.skolemize_injective; apply this
-    injection this with this
+    have := trg.apply_to_var_or_const_injective_of_not_in_frontier disj_index v_not_in_frontier (VarOrConst.var u)
+    rw [VarOrConst.var.injEq] at this
     rw [this]
-    exact u_in_frontier
+    . exact u_in_frontier
+    . rw [← u_eq, PreTrigger.apply_to_var_or_const_frontier_var]; exact u_in_frontier
+
 end PreTrigger
-
-structure LaxObsoletenessCondition (sig : Signature) [DecidableEq sig.P] [DecidableEq sig.C] [DecidableEq sig.V] where
-  cond : PreTrigger sig -> FactSet sig -> Prop
-  monotone : ∀ trg (A B : FactSet sig), A ⊆ B -> cond trg A -> cond trg B
-
-structure ObsoletenessCondition (sig : Signature) [DecidableEq sig.P] [DecidableEq sig.C] [DecidableEq sig.V] extends LaxObsoletenessCondition sig where
-  cond_implies_trg_is_satisfied : cond trg F -> trg.satisfied F
-  contains_trg_result_implies_cond : ∀ {trg : PreTrigger sig} {F} (disj_index : Fin trg.result.length), (trg.result.get disj_index) ⊆ F -> cond trg F
-
-instance {sig : Signature} [DecidableEq sig.P] [DecidableEq sig.C] [DecidableEq sig.V] : Coe (ObsoletenessCondition sig) (LaxObsoletenessCondition sig) where
-  coe obs := { cond := obs.cond, monotone := obs.monotone }
-
-def SkolemObsoleteness (sig : Signature) [DecidableEq sig.P] [DecidableEq sig.C] [DecidableEq sig.V] : ObsoletenessCondition sig := {
-  cond := fun (trg : PreTrigger sig) (F : FactSet sig) => ∃ i : Fin trg.mapped_head.length, (trg.mapped_head.get i).toSet ⊆ F
-  monotone := by
-    intro trg A B A_sub_B
-    simp
-    intro i head_sub_A
-    exists i
-    apply Set.subset_trans
-    . exact head_sub_A
-    . exact A_sub_B
-  cond_implies_trg_is_satisfied := by
-    intro trg F
-    simp
-    intro i h
-    exists ⟨i, by rw [← PreTrigger.length_mapped_head]; exact i.isLt⟩
-    exists (fun v => trg.apply_to_var_or_const i (VarOrConst.var v))
-    constructor
-    . intro v v_in_frontier
-      simp [PreTrigger.apply_to_var_or_const, PreTrigger.apply_to_skolemized_term, GroundSubstitution.apply_skolem_term, PreTrigger.skolemize_var_or_const, VarOrConst.skolemize, v_in_frontier]
-    . have : trg.mapped_head[i.val] = (trg.rule.head[i]'(by rw [← PreTrigger.length_mapped_head]; exact i.isLt)).map (fun a => { predicate := a.predicate, terms := a.terms.map (trg.apply_to_var_or_const i), arity_ok := (by rw [List.length_map, a.arity_ok])}) := by
-        unfold PreTrigger.mapped_head
-        unfold PreTrigger.apply_to_function_free_atom
-        simp
-        rfl
-      rw [this] at h
-
-      unfold GroundSubstitution.apply_function_free_conj
-      unfold GroundSubstitution.apply_function_free_atom
-
-      have : GroundSubstitution.apply_var_or_const (fun v => trg.apply_to_var_or_const i (VarOrConst.var v)) = trg.apply_to_var_or_const i := by
-        unfold GroundSubstitution.apply_var_or_const
-        apply funext
-        intro x
-        cases x with
-        | var => rfl
-        | const => simp [PreTrigger.apply_to_var_or_const, PreTrigger.apply_to_skolemized_term, GroundSubstitution.apply_skolem_term, PreTrigger.skolemize_var_or_const, VarOrConst.skolemize]
-      simp only [this]
-      apply h
-  contains_trg_result_implies_cond := by
-    intro trg F i result_in_F
-    unfold PreTrigger.result at result_in_F
-    simp at result_in_F
-    exists ⟨i, by have isLt := i.isLt; unfold PreTrigger.result at isLt; simp [List.length_map] at isLt; exact isLt⟩
-}
-
-def RestrictedObsoleteness (sig : Signature) [DecidableEq sig.P] [DecidableEq sig.C] [DecidableEq sig.V] : ObsoletenessCondition sig := {
-  cond := fun (trg : PreTrigger sig) (F : FactSet sig) => trg.satisfied F
-  monotone := by
-    intro trg A B A_sub_B
-    simp [PreTrigger.satisfied, PreTrigger.satisfied_for_disj]
-    intro i subs frontier_same_under_subs applied_head_sub_A
-    exists i
-    exists subs
-    constructor
-    . apply frontier_same_under_subs
-    . apply Set.subset_trans
-      . exact applied_head_sub_A
-      . exact A_sub_B
-  cond_implies_trg_is_satisfied := by intro _ _ h; exact h
-  contains_trg_result_implies_cond := by
-    intro trg F i result_in_F
-    let adjusted_i : Fin trg.rule.head.length := ⟨i, by rw [← PreTrigger.length_mapped_head]; have isLt := i.isLt; unfold PreTrigger.result at isLt; simp [List.length_map] at isLt; exact isLt⟩
-    let obs_subs := fun v : sig.V => trg.apply_to_var_or_const adjusted_i (VarOrConst.var v)
-
-    exists adjusted_i
-    exists obs_subs
-    constructor
-    . intro _ v'_in_frontier
-      simp [obs_subs, PreTrigger.apply_to_var_or_const, PreTrigger.apply_to_skolemized_term, PreTrigger.skolemize_var_or_const, GroundSubstitution.apply_skolem_term, VarOrConst.skolemize, v'_in_frontier]
-    . simp [obs_subs, GroundSubstitution.apply_function_free_conj]
-      unfold GroundSubstitution.apply_function_free_atom
-      intro f' hf'
-      apply result_in_F
-      unfold PreTrigger.result
-      unfold PreTrigger.mapped_head
-      unfold PreTrigger.apply_to_function_free_atom
-
-      have : ∀ (a : FunctionFreeAtom sig), (List.map (GroundSubstitution.apply_var_or_const obs_subs) a.terms) = (List.map (trg.apply_to_var_or_const adjusted_i) a.terms) := by
-        intro a
-        induction a.terms with
-        | nil => simp [List.map]
-        | cons head tail ih =>
-          simp [List.map, ih]
-          simp [obs_subs, GroundSubstitution.apply_skolem_term, GroundSubstitution.apply_var_or_const, PreTrigger.apply_to_var_or_const, PreTrigger.apply_to_skolemized_term, PreTrigger.skolemize_var_or_const]
-          cases head with
-          | var v => simp
-          | const c => simp [VarOrConst.skolemize]
-
-      simp
-      simp only [adjusted_i] at this
-      simp [← this]
-      apply hf'
-}
-
-variable {sig : Signature} [DecidableEq sig.P] [DecidableEq sig.C] [DecidableEq sig.V]
-
-structure Trigger (obsolete : LaxObsoletenessCondition sig) extends PreTrigger sig
-
-def SkolemTrigger := Trigger (SkolemObsoleteness sig : LaxObsoletenessCondition sig)
-def RestrictedTrigger := Trigger (RestrictedObsoleteness sig : LaxObsoletenessCondition sig)
-
-variable {obs : LaxObsoletenessCondition sig}
-
-instance : CoeOut (Trigger obs) (PreTrigger sig) where
-  coe trigger := { rule := trigger.rule, subs := trigger.subs }
-
-namespace Trigger
-  def active (trg : Trigger obs) (F : FactSet sig) : Prop :=
-    trg.loaded F ∧ ¬ (obs.cond trg F)
-end Trigger
-
-def RTrigger (obs : LaxObsoletenessCondition sig) (r : RuleSet sig) := { trg : Trigger obs // trg.rule ∈ r.rules}
-
-namespace RTrigger
-  def equiv (trg1 trg2 : RTrigger obs rs) : Prop := trg1.val.equiv trg2.val
-
-  theorem funcTermForExisVarInMultipleTriggersMeansTheyAreTheSame
-    {rs : RuleSet sig}
-    (trg1 trg2 : RTrigger obs rs)
-    (disjIndex1 : Fin trg1.val.rule.head.length)
-    (disjIndex2 : Fin trg2.val.rule.head.length)
-    (var1 var2 : sig.V)
-    (var1_not_in_frontier : ¬ var1 ∈ trg1.val.rule.frontier)
-    (var2_not_in_frontier : ¬ var2 ∈ trg2.val.rule.frontier)
-    :
-    (trg1.val.apply_to_var_or_const disjIndex1 (VarOrConst.var var1)) = (trg2.val.apply_to_var_or_const disjIndex2 (VarOrConst.var var2))
-    ->
-    trg1.equiv trg2 ∧ disjIndex1.val = disjIndex2.val := by
-    intro applications_eq
-    simp [PreTrigger.apply_to_var_or_const, PreTrigger.apply_to_skolemized_term, PreTrigger.skolemize_var_or_const, GroundSubstitution.apply_skolem_term, VarOrConst.skolemize, var1_not_in_frontier, var2_not_in_frontier, GroundTerm.func] at applications_eq
-    have rules_eq : trg1.val.rule = trg2.val.rule := by
-      apply rs.id_unique
-      constructor
-      exact trg1.property
-      constructor
-      exact trg2.property
-      exact applications_eq.left.left
-    constructor
-    . unfold equiv
-      unfold PreTrigger.equiv
-      constructor
-      . exact rules_eq
-      . let right := applications_eq.right
-        rw [← FiniteTreeList.eqIffFromListEq _ _] at right
-        have : trg1.val.rule.frontier = trg2.val.rule.frontier := by rw [rules_eq]
-        rw [← this] at right
-        rw [List.eq_iff_unattach_eq, List.map_eq_map_iff] at right
-        intro v v_mem
-        rw [List.mem_toSet] at v_mem
-        apply right
-        exact v_mem
-    . exact applications_eq.left.right.left
-end RTrigger
 
