ExistentialRules/Triggers/Obsoleteness.lean
@@ -1,0 +1,74 @@
+import ExistentialRules.Triggers.Basic
+
+structure LaxObsoletenessCondition (sig : Signature) [DecidableEq sig.P] [DecidableEq sig.C] [DecidableEq sig.V] where
+  cond : PreTrigger sig -> FactSet sig -> Prop
+  monotone : ∀ trg (A B : FactSet sig), A ⊆ B -> cond trg A -> cond trg B
+
+structure ObsoletenessCondition (sig : Signature) [DecidableEq sig.P] [DecidableEq sig.C] [DecidableEq sig.V] extends LaxObsoletenessCondition sig where
+  cond_implies_trg_is_satisfied : cond trg fs -> trg.satisfied fs
+  contains_trg_result_implies_cond : ∀ {trg : PreTrigger sig} {fs} (disj_index : Fin trg.mapped_head.length),
+    ((trg.mapped_head[disj_index.val]).toSet ⊆ fs) -> cond trg fs
+
+instance {sig : Signature} [DecidableEq sig.P] [DecidableEq sig.C] [DecidableEq sig.V] :
+    Coe (ObsoletenessCondition sig) (LaxObsoletenessCondition sig) where
+  coe obs := { cond := obs.cond, monotone := obs.monotone }
+
+def SkolemObsoleteness (sig : Signature) [DecidableEq sig.P] [DecidableEq sig.C] [DecidableEq sig.V] : ObsoletenessCondition sig := {
+  cond := fun (trg : PreTrigger sig) (fs : FactSet sig) => ∃ i : Fin trg.mapped_head.length, (trg.mapped_head[i.val]).toSet ⊆ fs
+  monotone := by
+    intro trg A B A_sub_B
+    simp
+    intro i head_sub_A
+    exists i
+    apply Set.subset_trans
+    . exact head_sub_A
+    . exact A_sub_B
+  cond_implies_trg_is_satisfied := by
+    intro trg fs h
+    rcases h with ⟨i, h⟩
+    exists ⟨i, by rw [← PreTrigger.length_mapped_head]; exact i.isLt⟩
+    apply trg.satisfied_for_disj_of_mapped_head_contained
+    exact h
+  contains_trg_result_implies_cond := by
+    intro trg F i result_in_F
+    exists i
+}
+
+def RestrictedObsoleteness (sig : Signature) [DecidableEq sig.P] [DecidableEq sig.C] [DecidableEq sig.V] : ObsoletenessCondition sig := {
+  cond := fun (trg : PreTrigger sig) (fs : FactSet sig) => trg.satisfied fs
+  monotone := by
+    intro trg A B A_sub_B
+    simp [PreTrigger.satisfied, PreTrigger.satisfied_for_disj]
+    intro i subs frontier_same_under_subs applied_head_sub_A
+    exists i
+    exists subs
+    constructor
+    . apply frontier_same_under_subs
+    . apply Set.subset_trans
+      . exact applied_head_sub_A
+      . exact A_sub_B
+  cond_implies_trg_is_satisfied := by intro _ _ h; exact h
+  contains_trg_result_implies_cond := by
+    intro trg fs i result_in_fs
+    exists ⟨i.val, by rw [← PreTrigger.length_mapped_head]; exact i.isLt⟩
+    apply trg.satisfied_for_disj_of_mapped_head_contained
+    exact result_in_fs
+}
+
+variable {sig : Signature} [DecidableEq sig.P] [DecidableEq sig.C] [DecidableEq sig.V]
+
+structure Trigger (obsolete : LaxObsoletenessCondition sig) extends PreTrigger sig
+
+def SkolemTrigger := Trigger (SkolemObsoleteness sig : LaxObsoletenessCondition sig)
+def RestrictedTrigger := Trigger (RestrictedObsoleteness sig : LaxObsoletenessCondition sig)
+
+variable {obs : LaxObsoletenessCondition sig}
+
+instance : CoeOut (Trigger obs) (PreTrigger sig) where
+  coe trigger := { rule := trigger.rule, subs := trigger.subs }
+
+namespace Trigger
+  def active (trg : Trigger obs) (F : FactSet sig) : Prop :=
+    trg.loaded F ∧ ¬ (obs.cond trg F)
+end Trigger
+
