ExistentialRules/Triggers/RTrigger.lean
@@ -1,0 +1,52 @@
+import ExistentialRules.Triggers.Obsoleteness
+
+variable {sig : Signature} [DecidableEq sig.P] [DecidableEq sig.C] [DecidableEq sig.V]
+variable {obs : LaxObsoletenessCondition sig}
+
+def RTrigger (obs : LaxObsoletenessCondition sig) (r : RuleSet sig) := { trg : Trigger obs // trg.rule ∈ r.rules}
+
+namespace RTrigger
+
+  def equiv (trg1 trg2 : RTrigger obs rs) : Prop := trg1.val.equiv trg2.val
+
+  theorem funcTermForExisVarInMultipleTriggersMeansTheyAreTheSame
+    {rs : RuleSet sig}
+    (trg1 trg2 : RTrigger obs rs)
+    (disjIndex1 : Fin trg1.val.rule.head.length)
+    (disjIndex2 : Fin trg2.val.rule.head.length)
+    (var1 var2 : sig.V)
+    (var1_not_in_frontier : ¬ var1 ∈ trg1.val.rule.frontier)
+    (var2_not_in_frontier : ¬ var2 ∈ trg2.val.rule.frontier)
+    :
+    (trg1.val.apply_to_var_or_const disjIndex1 (VarOrConst.var var1)) = (trg2.val.apply_to_var_or_const disjIndex2 (VarOrConst.var var2))
+    ->
+    trg1.equiv trg2 ∧ disjIndex1.val = disjIndex2.val := by
+    intro applications_eq
+    rw [PreTrigger.apply_to_var_or_const_non_frontier_var _ _ _ var1_not_in_frontier] at applications_eq
+    rw [PreTrigger.apply_to_var_or_const_non_frontier_var _ _ _ var2_not_in_frontier] at applications_eq
+    simp only [PreTrigger.functional_term_for_var, GroundTerm.func] at applications_eq
+    rw [Subtype.mk.injEq, FiniteTree.inner.injEq, SkolemFS.mk.injEq] at applications_eq
+    have rules_eq : trg1.val.rule = trg2.val.rule := by
+      apply rs.id_unique
+      constructor
+      . exact trg1.property
+      constructor
+      . exact trg2.property
+      . exact applications_eq.left.left
+    constructor
+    . unfold equiv
+      unfold PreTrigger.equiv
+      constructor
+      . exact rules_eq
+      . have right := applications_eq.right
+        rw [← FiniteTreeList.eqIffFromListEq _ _] at right
+        have : trg1.val.rule.frontier = trg2.val.rule.frontier := by rw [rules_eq]
+        rw [← this] at right
+        rw [List.eq_iff_unattach_eq, List.map_eq_map_iff] at right
+        intro v v_mem
+        apply right
+        exact v_mem
+    . exact applications_eq.left.right.left
+
+end RTrigger
+
